vcgen.lean
@@ -98,26 +98,26 @@ notation `⊢` σ `:` Q : 10 := env.vcgen σ Q
 
 notation `⊢` σ `:` Q : 10 := env.vcgen σ Q
 
-inductive stack.vcgen : stack → Prop
-notation `⊢ₛ` s : 10 := stack.vcgen s
+inductive stack.vcgen : callhistory → stack → Prop
+notation H `⊢ₛ` s : 10 := stack.vcgen H s
 
-| top {P: prop} {σ: env} {e: exp} {Q: propctx}:
+| top {H: callhistory} {P: prop} {σ: env} {e: exp} {Q: propctx}:
     (⊢ σ : P) →
-    (P ⊢ e : Q) →
-    (⊢ₛ (σ, e))
+    (H && P ⊢ e : Q) →
+    (H ⊢ₛ (σ, e))
 
-| cons {P: prop} {s: stack} {σ₁ σ₂: env} {f fx g x y: var} {R S: spec} {e: exp} {v: value} {Q: propctx}:
-    (⊢ₛ s) →
+| cons {H: callhistory} {P: prop} {s: stack} {σ₁ σ₂: env} {f fx g x y: var} {R S: spec} {e: exp} {v: value} {Q: propctx}:
+    (H ⊢ₛ s) →
     (⊢ σ₁ : P) →
     (σ₁ g = value.func f fx R S e σ₂) →
     (σ₁ x = v) →
     y ∉ σ₁ →
-    (P && prop.call g x && prop.post g x && (y ≡ term.app g x) ⊢ e : Q) →
-    ⟪ prop.implies (P && prop.call g x) (term.unop unop.isFunc g && prop.pre g x) ⟫ →
+    (H && P && prop.call g x && prop.post g x && (y ≡ term.app g x) ⊢ e : Q) →
+    ⟪ prop.implies (H && P && prop.call g x) (term.unop unop.isFunc g && prop.pre g x) ⟫ →
     ((σ₂[f↦value.func f fx R S e σ₂][fx↦v], e) ⟶* s) →
-    (⊢ₛ (s · [σ₁, let y = g[x] in e]))
+    (H ⊢ₛ (s · [σ₁, let y = g[x] in e]))
 
-notation `⊢ₛ` s : 10 := stack.vcgen s
+notation H `⊢ₛ` s : 10 := stack.vcgen H s
 
 -- lemmas
 
@@ -130,11 +130,11 @@ lemma exp.vcgen.return.inv {P: prop} {x: var} {Q: propctx}: (P ⊢ exp.return x 
     }
   end
 
-lemma stack.vcgen.top.inv {σ: env} {e: exp}: (⊢ₛ (σ, e)) → ∃P Q, (⊢ σ: P) ∧ (P ⊢ e: Q) :=
-  assume top_verified: ⊢ₛ (σ, e),
+lemma stack.vcgen.top.inv {H: callhistory} {σ: env} {e: exp}: (H ⊢ₛ (σ, e)) → ∃P Q, (⊢ σ: P) ∧ (H && P ⊢ e: Q) :=
+  assume top_verified: H ⊢ₛ (σ, e),
   begin
     cases top_verified,
     case stack.vcgen.top P Q env_verified e_verified {
-      show ∃P Q, (⊢ σ: P) ∧ (P ⊢ e: Q), from exists.intro P (exists.intro Q ⟨env_verified, e_verified⟩)
+      show ∃P Q, (⊢ σ: P) ∧ (H && P ⊢ e: Q), from exists.intro P (exists.intro Q ⟨env_verified, e_verified⟩)
     }
   end
