soundness.lean
@@ -2,19 +2,106 @@ import data.set
 
 import .syntax .notations .logic .evaluation .vcgen .progress .preservation
 
-theorem soundness {e: exp} {s: stack} {Q: propctx}:
-  (value.true ⊢ e: Q) → ((env.empty, e) ⟶* s) → (is_value s ∨ ∃s', s ⟶ s') :=
+lemma trivial_precondition:
+  ∀σ, σ ⊨ vc.implies (prop.instantiated_n (value.true && value.true)) (prop.instantiated_n (value.true)) :=
+  assume σ: env,
+  show σ ⊨ vc.implies (prop.instantiated_n (value.true && value.true)) (prop.instantiated_n (value.true)),
+  from valid_env.mpr (
+    assume _,
+    have h: σ ⊨ value.true, from valid_env.true,
+    have prop.erased (prop.term value.true) = vc.term value.true, by unfold prop.erased,
+    have σ ⊨ (prop.erased (value.true)), from this.symm ▸ h,
+    have σ ⊨ (prop.instantiated (value.true)), from valid_env.instantiated_of_erased this,
+    show σ ⊨ (prop.instantiated_n (value.true)), from valid_env.instantiated_n_of_instantiated this
+  )
+
+lemma trivial_freevars: FV (prop.term value.true && prop.term value.true) = FV (prop.term value.true) :=
+  have h1: FV (prop.term value.true && prop.term value.true) = ∅, from set.eq_empty_of_forall_not_mem (
+    assume x: var,
+    assume : x ∈ FV (prop.term value.true && prop.term value.true),
+    have x ∈ FV (prop.term value.true) ∨ x ∈ FV (prop.term value.true), from free_in_prop.and.inv this,
+    or.elim this (
+      assume : x ∈ FV (prop.term value.true),
+      have x ∈ FV (term.value value.true), from free_in_prop.term.inv this,
+      show «false», from free_in_term.value.inv this
+    ) (
+      assume : x ∈ FV (prop.term value.true),
+      have x ∈ FV (term.value value.true), from free_in_prop.term.inv this,
+      show «false», from free_in_term.value.inv this
+    )
+  ),
+  have h2: FV (prop.term value.true) = ∅, from set.eq_empty_of_forall_not_mem (
+    assume x: var,
+    assume : x ∈ FV (prop.term value.true),
+    have x ∈ FV (term.value value.true), from free_in_prop.term.inv this,
+    show «false», from free_in_term.value.inv this
+  ),
+  show FV (prop.term value.true && prop.term value.true) = FV (prop.term value.true), from eq.trans h1 h2.symm
+
+lemma trivial_calls: calls (prop.term value.true && prop.term value.true) = calls (prop.term value.true) :=
+  have h1: calls (prop.term value.true && prop.term value.true) = ∅, from set.eq_empty_of_forall_not_mem (
+    assume c: calltrigger,
+    assume : c ∈ calls (prop.term value.true && prop.term value.true),
+    have c ∈ calls (prop.term value.true) ∨ c ∈ calls (prop.term value.true), from has_call.and.inv this,
+    or.elim this (
+      assume : c ∈ calls (prop.term value.true),
+      show «false», from has_call.term.inv this
+    ) (
+      assume : c ∈ calls (prop.term value.true),
+      show «false», from has_call.term.inv this
+    )
+  ),
+  have h2: calls (prop.term value.true) = ∅, from set.eq_empty_of_forall_not_mem (
+    assume c: calltrigger,
+    assume : c ∈ calls (prop.term value.true),
+    show «false», from has_call.term.inv this
+  ),
+  show calls (prop.term value.true && prop.term value.true) = calls (prop.term value.true), from eq.trans h1 h2.symm
+
+lemma trivial_quantifiers: quantifiers (prop.term value.true && prop.term value.true) = quantifiers (prop.term value.true) :=
+  have h1: quantifiers (prop.term value.true && prop.term value.true) = ∅, from set.eq_empty_of_forall_not_mem (
+    assume q: callquantifier,
+    assume : q ∈ quantifiers (prop.term value.true && prop.term value.true),
+    have q ∈ quantifiers (prop.term value.true) ∨ q ∈ quantifiers (prop.term value.true), from has_quantifier.and.inv this,
+    or.elim this (
+      assume : q ∈ quantifiers (prop.term value.true),
+      show «false», from has_quantifier.term.inv this
+    ) (
+      assume : q ∈ quantifiers (prop.term value.true),
+      show «false», from has_quantifier.term.inv this
+    )
+  ),
+  have h2: quantifiers (prop.term value.true) = ∅, from set.eq_empty_of_forall_not_mem (
+    assume q: callquantifier,
+    assume : q ∈ quantifiers (prop.term value.true),
+    show «false», from has_quantifier.term.inv this
+  ),
+  show quantifiers (prop.term value.true && prop.term value.true) = quantifiers (prop.term value.true), from eq.trans h1 h2.symm
+
+lemma soundness {s s': stack}: (s ⟶* s') → ∀H, (H ⊢ₛ s) → (is_value s' ∨ ∃h s'', s' ⟶ h, s'') :=
+  assume steps_to_s': s ⟶* s',
+  begin
+    induction steps_to_s',
+    case trans_step.rfl s₁ {
+      assume H,
+      assume s₁_verified ,
+      show is_value s₁ ∨ ∃h s', s₁ ⟶ h, s', from progress H s₁ s₁_verified
+    },
+    case trans_step.trans s₁ s₂ s₃ h s₁_steps_to_s₂ s₂_steps_to_s₃ ih {
+      assume H,
+      assume s₁_verified ,
+      have : (h :: H ⊢ₛ s₂), from preservation s₁_verified s₁_steps_to_s₂,
+      show is_value s₃ ∨ ∃h s', s₃ ⟶ h, s', from ih (h::H) this
+    }
+  end
+
+theorem soundness_source_programs {e: exp} {s: stack} {Q: propctx}:
+  (value.true ⊢ e: Q) → ((env.empty, e) ⟶* s) → (is_value s ∨ ∃h s', s ⟶ h, s') :=
 
   assume initial_verified: value.true ⊢ e: Q,
   assume steps_to_s: (env.empty, e) ⟶* s,
-  have h: ⊢ₛ (env.empty, e), from stack.vcgen.top env.vcgen.empty initial_verified,
-  begin
-    induction steps_to_s,
-    case trans_step.rfl s₁ {
-      show is_value s₁ ∨ ∃s', s₁ ⟶ s', from progress h
-    },
-    case trans_step.trans s₁ s₂ s₃ s₁_steps_to_s₂ s₂_steps_to_s₃ ih {
-      have : ⊢ₛ s₂, from preservation h s₁_steps_to_s₂,
-      show is_value s₃ ∨ ∃s', s₃ ⟶ s', from ih this
-    }
-  end
+  have (prop.term value.true && prop.term value.true) ⊢ e: Q,
+  from strengthen_pre_exp initial_verified (prop.term value.true && prop.term value.true)
+       trivial_freevars trivial_calls trivial_quantifiers trivial_precondition,
+  have list.nil ⊢ₛ (env.empty, e), from stack.vcgen.top env.vcgen.empty this,
+  show is_value s ∨ ∃h s', s ⟶ h, s', from soundness steps_to_s list.nil this
